pulse/share/steel/examples/pulse/dice/lib/PulseHashTable.fst
@@ -1,0 +1,55 @@
+module PulseHashTable
+module PM = Pulse.Main
+open Steel.ST.Array
+open Steel.FractionalPermission
+open Steel.ST.Util
+open FStar.Ghost
+open Pulse.Steel.Wrapper
+module A = Steel.ST.Array
+module R = Steel.ST.Reference
+module US = FStar.SizeT
+module U8 = FStar.UInt8
+module LK = Steel.ST.SpinLock
+module PHT = LinearScanHashTable
+open LinearScanHashTable
+
+noeq
+type ht (s : pht_sig) = {
+  sz : pos;
+  contents : A.larray (cell s.keyt s.valt) sz;
+}
+
+let models (s:pht_sig) (pht:pht s) (ht:ht s) : vprop
+= A.pts_to ht.contents full_perm pht.repr `star`
+  pure (pht.sz == ht.sz)
+
+```pulse
+fn insert (#s:pht_sig) (#pht:(p:pht s{not_full p.repr})) 
+          (table:ht s) (k:s.keyt) (v:s.valt)
+  requires models s pht table
+  ensures  models s (PHT.insert pht k v) table
+{
+  admit()
+}
+```
+
+```pulse
+fn delete (#s:pht_sig) (#pht:(p:pht s{not_full p.repr})) 
+          (table:ht s) (k:s.keyt)
+  requires models s pht table
+  ensures  models s (PHT.delete pht k) table
+{
+  admit()
+}
+```
+
+```pulse
+fn lookup (#s:pht_sig) (#pht:(p:pht s{not_full p.repr})) 
+          (table:ht s) (k:s.keyt)
+  requires models s pht table
+  returns  o:option s.valt
+  ensures  models s pht table
+{
+  admit()
+}
+```
